

Name of the Examination : First Semester End Semester Examination

Name of the Subject : Mathematics

Subject Code : MA1101

Date of Examination : 30<sup>th</sup> March, 2021

Name of the Student : Tathagata Ghosh

Examination Roll Number : 2020ITB065

G Suite ID : [2020ITB065.tathagata@students.iests.ac.in](mailto:2020ITB065.tathagata@students.iests.ac.in)

Number of Sheets uploaded : 11

Ans) Let  $f(x) = \sin x$

Therefore,  $f(0) = 0$

$$f'(x) = \cos x \quad ; \quad f'(0) = 1$$

$$f''(x) = -\sin x \quad ; \quad f''(0) = 0$$

$$f'''(x) = -\cos x \quad ; \quad f'''(\theta x) = -\cos \theta x$$

Now, the Maclaurin's series for the function  $f(x)$  with Lagrange's form of remainder after three term is

$$f(x) = f(0) + x f'(0) + \frac{x^2}{2!} f''(0) + \frac{x^3}{3!} f'''(\theta x), \quad 0 < \theta < 1$$

$$\therefore \sin x = x - \frac{x^3}{3!} \cos \theta x = x - \frac{x^3}{6} \cos \theta x \quad \dots \dots (1)$$

$$\text{Now, } 0 < x < \frac{\pi}{2} \text{ and } 0 < \theta < 1$$

$$\Rightarrow 0 < \theta x < \frac{\pi}{2}$$

$$\Rightarrow 0 < \cos \theta x < 1$$

$$\therefore \frac{x^3}{6} \cos \theta x < \frac{x^3}{6}$$

$$\Rightarrow -\frac{x^3}{6} \cos \theta x > -\frac{x^3}{6}$$

$$\Rightarrow x - \frac{x^3}{6} \cos \theta x > x - \frac{x^3}{6}$$

$$\therefore \sin x > x - \frac{1}{6} x^3 \quad \dots \dots [\text{by } (1)]$$

$$\text{if } 0 < x < \frac{\pi}{2} \quad (\text{Hence proved})$$

Name of the Examination : First Semester End Semester Examination  
 Name of the Subject : Mathematics  
 Subject Code : MA1101  
 Date of Examination : 30<sup>th</sup> March, 2021  
 Name of the Student : Tathagata Ghosh  
 Examination Roll Number : 2020ITB065  
 G Suite ID : [2020ITB065.tathagata@students.iests.ac.in](mailto:2020ITB065.tathagata@students.iests.ac.in)  
 Number of Sheets uploaded : 11

Ans 1b) Given,  $x = a(\theta + \sin\theta)$   $y = a(1 - \cos\theta)$   
[Differentiating both sides w.r.t  $\theta$ ] [Differentiating both sides w.r.t  $\theta$ ]  
 $\Rightarrow x' = a(1 + \cos\theta)$   $y' = a \sin\theta$   
[Differentiating both sides w.r.t  $\theta$ ] [Differentiating both sides w.r.t  $\theta$ ]  
 $x'' = -a \sin\theta$   $y'' = a \cos\theta$

$\therefore$  Radius of curvature

$$\begin{aligned} \rho &= \frac{(x'^2 + y'^2)^{3/2}}{x'y'' - y'x''} \quad (\text{Parametric form}) \\ &= \frac{[a^2(1 + \cos\theta)^2 + a^2 \sin^2\theta]^{3/2}}{a^2(\cos\theta + \cos^3\theta) + a^2 \sin^2\theta} \\ &= \frac{(2a^2 + 2a^2 \cos\theta)^{3/2}}{a^2 + a^2 \cos\theta} \\ &= 2\sqrt{2} (a^2 + a^2 \cos\theta)^{1/2} \\ &= 2\sqrt{2} a (2\cos^2\theta/2)^{1/2} \\ &= 4a \cos \frac{\theta}{2} \quad (\text{Ans}) \end{aligned}$$

Ans 1c) Equating the coefficient of highest power of  $x$  i.e;  $x^2$  equal to zero, horizontal asymptotes are given by

$y^2 - y = 0 \Rightarrow y(y-1) = 0$  i.e;  $y = 0, y = 1$   
 Equating coefficient of highest power of  $y$ , i.e;  $y^2$  equal to zero, vertical asymptotes are given by

$$\begin{aligned} x^2 - x &= 0 \quad \text{i.e; } x = 0, x = 1 \\ \Rightarrow x(x-1) &= 0 \end{aligned}$$

Name of the Examination : First Semester End Semester Examination

Name of the Subject : Mathematics

Subject Code : MA1101

Date of Examination : 30<sup>th</sup> March, 2021

Name of the Student : Tathagata Ghosh

Examination Roll Number : 2020ITB065

G Suite ID : 2020ITB065.tathagata@students.iiests.ac.in

Number of Sheets uploaded : 11

Given equation is 4th degree equation in  $x$  and  $y$  and hence curve cannot have more than 4 asymptotes.

$\therefore$  All asymptotes are  $y=0, y=1, x=0, x=1$ .

Ans 2a) ii)  $u_n = \frac{n^p}{n!}, u_{n+1} = \frac{(n+1)^p}{(n+1)!}$

$$\frac{u_{n+1}}{u_n} = \frac{(n+1)^p}{(n+1)!} \times \frac{n!}{n^p} = \frac{1}{(n+1)} \left(1 + \frac{1}{n}\right)^p$$

$$\lim_{n \rightarrow \infty} \frac{u_{n+1}}{u_n} = \lim_{n \rightarrow \infty} \left\{ \frac{1}{(n+1)} \cdot \left(1 + \frac{1}{n}\right)^p \right\}$$

$$= 0 < 1$$

$\therefore$  The series is convergent by D'Alembert's Test.

Ans 2a) iii)  $a_n = \frac{n^3+a}{2^n+a}, b_n = \frac{n^3}{2^n}$

$$\frac{a_n}{b_n} = \frac{n^3+a}{2^n+a} \times \frac{2^n}{n^3}$$

$$= \left(1 + \frac{a}{n^3}\right) \left(\frac{2^n}{2^n+a}\right)$$

$$= \left(1 + \frac{a}{n^3}\right) \left(\frac{1}{1 + \frac{a}{2^n}}\right)$$

$$\lim_{n \rightarrow \infty} \frac{a_n}{b_n} = 1$$

$\therefore$  By comparison test the given series is convergent or divergent according as  $\sum \frac{n^3}{2^n}$  is convergent or divergent.



Name of the Examination : First Semester End Semester Examination  
 Name of the Subject : Mathematics  
 Subject Code : MA1101  
 Date of Examination : 30<sup>th</sup> March, 2021  
 Name of the Student : Tathagata Ghosh  
 Examination Roll Number : 2020ITB065  
 G Suite ID : [2020ITB065.tathagata@students.iests.ac.in](mailto:2020ITB065.tathagata@students.iests.ac.in)  
 Number of Sheets uploaded : 4

respectively.

By Cauchy's Root Test,  
 $\lim_{n \rightarrow \infty} (b_n)^{\frac{1}{n}} = \lim_{n \rightarrow \infty} \frac{n^{\frac{3}{n}}}{2} = \frac{1}{2} < 1$

$\sum_{n=0}^{\infty} b_n$  is convergent  $\rightarrow \sum_{n=0}^{\infty} a_n$  is also convergent.

Ans 2b)  $\sum_{n=1}^{\infty} \frac{2^n}{n^2} (x-3)^n$   $u_{n+1} = \frac{2^{n+1}}{(n+1)^2} (x-3)^{n+1}$   
 $u_n = \frac{2^n}{n^2} (x-3)^n$

$\lim_{n \rightarrow \infty} \left| \frac{u_{n+1}}{u_n} \right| = \lim_{n \rightarrow \infty} |x-3| \cdot 2 \cdot \frac{n^2+2n+1}{n^2}$  [By D'Alembert's Test]  
 $= 2|x-3| \lim_{n \rightarrow \infty} \frac{n^2+2n+1}{n^2}$   
 $= 2|x-3|$

So, the series converges,

for  $|x-3| < \frac{1}{2}$  i.e;  $\frac{5}{2} < x < \frac{7}{2}$

at  $x = \frac{5}{2}$   $\sum_{n=1}^{\infty} \frac{2^n}{n^2} \left(-\frac{1}{2}\right)^n = \sum_{n=1}^{\infty} \frac{(-1)^n}{n^2}$  (convergent)

So, the original series is convergent

when  $x = \frac{7}{2}$ ,  $\sum_{n=1}^{\infty} \frac{2^n}{n^2} \left(\frac{1}{2}\right)^n = \sum_{n=1}^{\infty} \frac{1}{n^2}$  (convergent)

Hence, the interval of convergence is  $[\frac{5}{2}, \frac{7}{2}]$

radius of curvature,  $r = \left| \frac{a_{n+1}}{a_n} \right|$   
 $= 2 \cdot \frac{n^2+2n+1}{n^2} = 2$  (Ans)

Name of the Examination : First Semester End Semester Examination

Name of the Subject : Mathematics

Subject Code : MA1101

Date of Examination : 30<sup>th</sup> March, 2021

Name of the Student : Tathagata Ghosh

Examination Roll Number : 2020ITB065

G Suite ID : [2020ITB065.tathagata@students.iests.ac.in](mailto:2020ITB065.tathagata@students.iests.ac.in)

Number of Sheets uploaded : 11

Ans 2a)  $u = f(x, y)$  ;  $x = r \cos \theta$   $y = r \sin \theta$  (given)

$$\frac{\partial x}{\partial r} = \cos \theta \quad \frac{\partial y}{\partial r} = \sin \theta$$

$$\frac{\partial x}{\partial \theta} = -r \sin \theta \quad \frac{\partial y}{\partial \theta} = r \cos \theta$$

$$\frac{\partial u}{\partial r} = \frac{\partial u}{\partial x} \times \frac{\partial x}{\partial r} + \frac{\partial u}{\partial y} \times \frac{\partial y}{\partial r}$$

$$\Rightarrow \frac{\partial u}{\partial r} = \frac{\partial u}{\partial x} \cos \theta + \frac{\partial u}{\partial y} \sin \theta \quad \dots \text{--- (1)}$$

$$\boxed{\frac{\partial}{\partial r} = \cos \theta \frac{\partial}{\partial x} + \sin \theta \frac{\partial}{\partial y}}$$

Also  $\frac{\partial u}{\partial \theta} = \frac{\partial u}{\partial x} \times \frac{\partial x}{\partial \theta} + \frac{\partial u}{\partial y} \times \frac{\partial y}{\partial \theta}$

$$\Rightarrow \frac{\partial u}{\partial \theta} = -r \sin \theta \frac{\partial u}{\partial x} + r \cos \theta \frac{\partial u}{\partial y}$$

$$\boxed{\frac{\partial}{\partial \theta} = -r \sin \theta \frac{\partial}{\partial x} + r \cos \theta \frac{\partial}{\partial y}}$$

R.H.S

$$\left(\frac{\partial u}{\partial r}\right)^2 + \frac{1}{r^2} \left(\frac{\partial u}{\partial \theta}\right)^2 = \left(\cos \theta \frac{\partial u}{\partial x} + \sin \theta \frac{\partial u}{\partial y}\right)^2 +$$

$$\frac{1}{r^2} \left(-r \sin \theta \frac{\partial u}{\partial x} + r \cos \theta \frac{\partial u}{\partial y}\right)^2$$

$$= (\cos^2 \theta + \sin^2 \theta) \left(\frac{\partial u}{\partial x}\right)^2 + (\sin^2 \theta + \cos^2 \theta) \left(\frac{\partial u}{\partial y}\right)^2$$

$$= \left(\frac{\partial u}{\partial x}\right)^2 + \left(\frac{\partial u}{\partial y}\right)^2 = \text{L.H.S (Hence proved)}$$

Name of the Examination : First Semester End Semester Examination

Name of the Subject : Mathematics

Subject Code : MA1101

Date of Examination : 30<sup>th</sup> March, 2021

Name of the Student : Tathagata Ghosh

Examination Roll Number : 2020ITB065

G Suite ID : [2020ITB065.tathagata@students.iists.ac.in](mailto:2020ITB065.tathagata@students.iists.ac.in)

Number of Sheets uploaded : 1)

Ans 3b)  $V = \cos^{-1} \left( \frac{x+y}{\sqrt{x} + \sqrt{y}} \right)$

Let  $u = \cos V$

$$\Rightarrow u = \sqrt{x} \left( \frac{1 + \frac{y}{x}}{1 + \sqrt{\frac{y}{x}}} \right)$$

$$\Rightarrow u = \sqrt{x} \phi \left( \frac{y}{x} \right) \quad \dots \text{Degree } n = \frac{1}{2} ; \text{homogeneous equation}$$

Using Euler's Theorem,

$$x \frac{\partial u}{\partial x} + y \frac{\partial u}{\partial y} = \frac{1}{2} u \quad [\because n = \frac{1}{2}]$$

$$\Rightarrow x \frac{\partial (\cos V)}{\partial x} + y \frac{\partial (\cos V)}{\partial y} = \frac{1}{2} \cos V \quad [\because u = \cos V]$$

$$\Rightarrow -x \sin V \frac{\partial V}{\partial x} + -y \sin V \frac{\partial V}{\partial y} = \frac{1}{2} (\cos V)$$

$$\Rightarrow x \frac{\partial V}{\partial x} + y \frac{\partial V}{\partial y} + \frac{1}{2} \cot V = 0$$

Ans 4a)  $f_{xy} = \begin{cases} xy \frac{x^2 - y^2}{x^2 + y^2} & ; x^2 + y^2 \neq 0 \\ 0 & ; x^2 + y^2 = 0 \end{cases} \quad (\text{given})$

$$f_{xy}(0,0) = \lim_{h \rightarrow 0} \frac{f_y(0+h,0) - f_y(0,0)}{h} \left[ \frac{\partial f_y}{\partial x} \right]_{\substack{\text{at } x=0 \\ y=0}}$$

$$f_{xy}(0,0) = \lim_{h \rightarrow 0} \frac{f_y(h,0) - f_y(0,0)}{h} \quad \text{--- (1)}$$

Now,  $f_y(h,0) = \frac{\partial f}{\partial y} \Big|_{\text{at } x=h, y=0}$

Name of the Examination : First Semester End Semester Examination

Name of the Subject : Mathematics

Subject Code : MA1101

Date of Examination : 30<sup>th</sup> March, 2021

Name of the Student : Tathagata Ghosh

Examination Roll Number : 2020ITB065

G Suite ID : [2020ITB065.tathagata@students.iiests.ac.in](mailto:2020ITB065.tathagata@students.iiests.ac.in)

Number of Sheets uploaded : 11

$$= \lim_{k \rightarrow 0} \frac{f(h, k) - f(h, 0)}{k}$$

$$= \lim_{k \rightarrow 0} \frac{h \cancel{k} \frac{h^2 - k^2}{h^2 + k^2} - 0}{k}$$

$$= \lim_{k \rightarrow 0} h \left( \frac{h^2 - k^2}{h^2 + k^2} \right) = \frac{h^3}{h} = h \quad \text{--- (2)}$$

$$f_y(0, 0) = \left. \frac{\partial f}{\partial y} \right|_{\text{at } x=0, y=0}$$

$$= \lim_{k \rightarrow 0} \frac{f(0, k) - f(0, 0)}{k} = \lim_{k \rightarrow 0} \frac{0 - 0}{k} = 0 \quad \text{--- (3)}$$

From (1),

$$f_{xy}(0, 0) = \lim_{h \rightarrow 0} \frac{f_y(h, 0) - f_y(0, 0)}{h}$$

$$= \lim_{h \rightarrow 0} \frac{h - 0}{h} \quad [\text{By (2) \& (3)}]$$

= 1

$$\text{Again ; } f_{yx}(0, 0) = \left. \frac{\partial}{\partial y} f_x \right|_{\text{at } x=0, y=0}$$

$$= \lim_{k \rightarrow 0} \frac{f_x(0, k) - f_x(0, 0)}{k} \quad \text{--- (4)}$$

$$\text{Now, } f_x(0, k) = \left. \frac{\partial f}{\partial x} \right|_{\text{at } x=0, y=k}$$

$$= \lim_{h \rightarrow 0} \frac{f(h, k) - f(0, k)}{h}$$

$$= \lim_{h \rightarrow 0} \frac{h \cancel{k} \frac{h^2 - k^2}{h^2 + k^2} - 0}{h}$$



Name of the Examination : First Semester End Semester Examination

Name of the Subject : Mathematics

Subject Code : MA1101

Date of Examination : 30<sup>th</sup> March, 2021

Name of the Student : Tathagata Ghosh

Examination Roll Number : 2020ITB065

G Suite ID : 2020ITB065.tathagata@students.iests.ac.in

Number of Sheets uploaded : 11

$$\lim_{h \rightarrow 0} \frac{1}{h} \cdot k \frac{h^2 - k^2}{h^2 + k^2} = \lim_{h \rightarrow 0} \frac{h^2 k - k^3}{h^2 + k^2} = \frac{-k^3}{k^2} = -k \dots \textcircled{5}$$
$$f_x(0,0) = \left. \frac{\partial f}{\partial x} \right|_{\text{at } x=0, y=0} = \lim_{h \rightarrow 0} \frac{f(h,0) - f(0,0)}{h}$$

Using  $\textcircled{5}$  &  $\textcircled{6}$  in  $\textcircled{4}$ , we get

$$f_{yx}(0,0) = \lim_{k \rightarrow 0} \frac{f_x(0,k) - f_x(0,0)}{k}$$
$$= \lim_{k \rightarrow 0} \frac{-k - 0}{k} = -1$$

$\therefore f_{xy}(0,0) \neq f_{yx}(0,0)$  (Hence proved)

Ans 4b)

$$\int_0^{\infty} \frac{x^2 dx}{4x^4 + 25} \quad f(x) = \frac{x^2}{4x^4 + 25}$$

Let  $\mu = 2$

$$\lim_{x \rightarrow \infty} x^{\mu} \frac{x^2}{4x^4 + 25} = \lim_{x \rightarrow \infty} \frac{x^4}{4x^4 + 25} = \lim_{x \rightarrow \infty} \frac{1}{4 + \frac{25}{x^4}}$$
$$= \frac{1}{4} \text{ (finite)}$$

here  $\mu = 2 > 1$

$\therefore$  By  $\mu$ -test the integral is convergent.

Ans 4c)  $\Gamma(n+1)$

$$= \int_0^{\infty} e^{-x} x^{n+1-1} dx = \int_0^{\infty} e^{-x} x^n dx$$
$$= \lim_{b \rightarrow \infty} \int_0^b e^{-x} x^n dx$$
$$= \lim_{b \rightarrow \infty} \left[ \frac{e^{-x}}{-1} x^n \right]_0^b - \int_0^b \frac{e^{-x}}{-1} \cdot n x^{n-1} dx$$



Name of the Examination : First Semester End Semester Examination  
 Name of the Subject : Mathematics  
 Subject Code : MA1101  
 Date of Examination : 30<sup>th</sup> March, 2021  
 Name of the Student : Tathagata Ghosh  
 Examination Roll Number : 2020ITB065  
 G Suite ID : 2020ITB065.tathagata@students.iests.ac.in  
 Number of Sheets uploaded : 11

$$= \lim_{b \rightarrow \infty} \left[ e^{-b} b^n + n \int_0^b e^{-x} x^{n-1} dx \right]$$

$$= \lim_{b \rightarrow \infty} \frac{b^n}{e^b} + n \lim_{b \rightarrow \infty} \int_0^b e^{-x} x^{n-1} dx$$

$$= 0 + n \int_0^{\infty} e^{-x} x^{n-1} dx$$

$$= n \Gamma'(n) \quad [\text{proved}] \quad \left[ \because \int_0^{\infty} e^{-x} x^{n-1} dx = \Gamma'(n) \right]$$

Ans a)  $\frac{d^2 y}{dx^2} - 3 \frac{dy}{dx} + 2y = \frac{e^x}{1+e^x}$

$$(D^2 - 3D + 2)y = \frac{e^x}{1+e^x}$$

where  $R = \frac{e^x}{1+e^x}$

Auxiliary Equation is  $m^2 - 3m + 2 = 0 \Rightarrow m = 1, 2$  so

Complementary Function  $= C_1 e^x + C_2 e^{2x}$

Hence parts of C.F. are  $u = e^x$ ,  $v = e^{2x}$

$$\Rightarrow W = \begin{vmatrix} u & v \\ u' & v' \end{vmatrix} = e^{3x}$$

$$A = - \int \frac{Rv}{W} dx = - \int \frac{e^x \cdot e^{2x}}{(1+e^x)e^{3x}} dx = - \int \frac{e^{-x}}{e^{-x}+1} dx = \log(e^{-x}+1)$$

$$B = \int \frac{Ru}{W} dx = \int \left( \frac{e^x}{1+e^x} \cdot \frac{e^x}{e^{3x}} \right) dx = \int \frac{1}{e^x(e^x+1)} dx$$

$$= \int \left( \frac{1}{e^x} - \frac{1}{e^x+1} \right) dx$$

$$= \int \left( e^{-x} - \frac{e^{-x}}{e^{-x}+1} \right) dx = -e^{-x} + \log(e^x+1)$$

Name of the Examination : First Semester End Semester Examination

Name of the Subject : Mathematics

Subject Code : MA1101

Date of Examination : 30<sup>th</sup> March, 2021

Name of the Student : Tathagata Ghosh

Examination Roll Number : 2020ITB065

G Suite ID : [2020ITB065.tathagata@students.iests.ac.in](mailto:2020ITB065.tathagata@students.iests.ac.in)

Number of Sheets uploaded : 11

So, by variation of parameters, general solution is

$$\begin{aligned} y &= c_1 f + P \int (c_1 u + c_2 v) + (Au + Bv) \\ &= c_1 e^x + c_2 e^{2x} + (\log(e^x + 1)) \cdot e^x + \\ &\quad \{ -e^{-x} + \log(e^{-x} + 1) \} \cdot e^{2x} \end{aligned}$$

Ans b)  $P_n(x) = \frac{1}{n! 2^n} \frac{d^n}{dx^n} (x^2 - 1)^n$

Here let  $v = (x^2 - 1)^n \Rightarrow v_1 = \frac{dv}{dx} = 2nx(x^2 - 1)^{n-1}$

i.e;  $(1 - x^2)v_1 + 2nxv = 0$  --- (1)

Differentiating  $(n+1)$  times using Leibnitz rule,

$$\begin{aligned} (1 - x^2)v_{n+2} + (n+1)(-2x)v_{n+1} + \frac{1}{2!}(n+1)n(-2)v_n \\ + 2n[xv_{n+1} + (n+1)v_n] = 0 \end{aligned}$$

$$\Rightarrow (1 - x^2) \frac{d^2(v_n)}{dx^2} - 2x \frac{d(v_n)}{dx} + n(n+1)v_n = 0$$

It is the Legendre equation and  $c v_n$  is its solution. Also its finite series solution is  $P_n(x)$ .

$$P_n(x) = c v_n = c \frac{d^n}{dx^n} (x^2 - 1)^n \text{ --- (2)}$$

For finding the constant  $c$ , putting  $x=1$ ,

$$\begin{aligned} \text{then } 1 &= c \left[ \frac{d^n}{dx^n} \{ (x-1)^n (x+1)^n \} \right]_{x=1} \\ &= c [n! (n+1)^n] \end{aligned}$$

Also, it contains the terms of  $(x-1)$  and its powers  $|x=1$

Name of the Examination : First Semester End Semester Examination

Name of the Subject : Mathematics

Subject Code : MA1101

Date of Examination : 30<sup>th</sup> March, 2021

Name of the Student : Tathagata Ghosh

Examination Roll Number : 2020ITB065

G Suite ID : [2020ITB065.tathagata@students.iiests.ac.in](mailto:2020ITB065.tathagata@students.iiests.ac.in)

Number of Sheets uploaded : 11

$$= c \cdot n! \cdot 2^n ; \text{ i.e.; } c = \frac{1}{n!} 2^n$$

Substituting this value of  $c$  in (2), we get  
 (1) which proves that  $P_n(x) = \frac{1}{2^n n!} \cdot \frac{d^n}{dx^n} (x^2-1)^n$   
 (hence proved)

T. Ghosh